compression/compression.dfy
@@ -51,12 +51,27 @@ method {:main} Main(ghost env:HostEnvironment?)
   modifies env.ok;
   modifies env.files;
 {
+  /*var alo := ArrayFromSeq([0,1,2,3,4,0,1,2]);
+  var buffe: array<byte>, position: int := alo, 5;
+  if 0 < position < buffe.Length {
+    var match_: bool, offset: int, size: int := LZSS.LongestMatch(buffe, position);
+    print(match_);
+    print("\n");
+    print(offset);
+    print("\n");
+    print(size);
+    print("\n");
+    return;
+  }*/
+  
   var argc := HostConstants.NumCommandLineArgs(env);
+
   if argc != 4 {
-    print "[USAGE]: mono cp.exe SrcFilename DstFilename!\n";
+    print "[USAGE]: mono {0=Compress,1=Decompress} cp.exe SrcFilename DstFilename!\n";
     return;
   }
   
+  var act := HostConstants.GetCommandLineArg(1, env);
   var src := HostConstants.GetCommandLineArg(2, env);
   var dst := HostConstants.GetCommandLineArg(3, env);
 
@@ -71,6 +86,7 @@ method {:main} Main(ghost env:HostEnvironment?)
     print "Failed to open src file!\n";
     return;
   }
+
   var dstSuccess, dstFs := FileStream.Open(dst, env);
   if !dstSuccess {
     print "Failed to open dst file!\n";
@@ -86,66 +102,63 @@ method {:main} Main(ghost env:HostEnvironment?)
   var buffer := new byte[len];
   var srcOk := srcFs.Read(0 as nat32, buffer, 0, len);
   if !srcOk {return;}
-  /*var l := 0;
-  while l < buffer.Length
-    decreases buffer.Length - l
+  
+  var to: seq<byte> := LZSS.Encode(buffer);
+  var toTmp := ArrayFromSeq(to);
+  var to1: seq<byte> := LZSS.Decode(toTmp);
+  
+  var i := 0;
+  while i < buffer.Length && i < |to1| && i < |to|
+    decreases |to1| - i
   {
-    print(buffer[l]);
-    print("-");
-    l := l + 1;
-  }
-  print("\n");*/
-  var to: array<byte>, toSize: int := LZSS.Encode(buffer);
-  /*var i := 0;
-  while i < toSize && i < to.Length
-    decreases to.Length - i
-  {
-    print(to[i]);
-    print("-");
+    if buffer[i] != to1[i] {
+      print("(");
+      print(i);
+      print(",");
+      print(buffer[i]);
+      print(",");
+      print(to[i]);
+      print(",");
+      print(to1[i]);
+      print(")");
+      print("\n");
+      break;
+    }
     i := i + 1;
   }
-  print("\n");*/
-  
-  if 0 < toSize < to.Length {
-    var a := ArrayFromSeq(to[0..toSize]);
-    var to1: array<byte>, toSize1: int := LZSS.Decode(a);
-    if 0 < toSize1 < to1.Length {
-      to1 := ArrayFromSeq(to1[0..toSize1]);
-    }
-    var i := 0;
-    if buffer.Length != to1.Length {return;}
-    
-    while i < to1.Length
-      decreases to1.Length - i
-    {
-      //print(to1[i]);
-      //print("-");
-      if buffer[i] != to1[i] {
-        print("(");
-        print(i);
-        print(",");
-        print(buffer[i]);
-        print(",");
-        print(to1[i]);
-        print(")");
-        print("\n");
-      
-        //break;
-      }
-      i := i + 1;
-    }
     print("\n");
     print("(");
     print(buffer.Length);
     print(",");
-    print(a.Length);
+    print(|to|);
     print(",");
-    print(to1.Length);
+    print(|to1|);
     print(")\n");
-
-    var dstOk := dstFs.Write(0 as nat32, to1, 0, to1.Length as int32);
-    //if dstOk {
-    //  var a := dstFs.Close();
-    //}
   }
+  /*if act.Length != 1 {return;}
+  var to: array<byte>, toSize: int, dstOk;
+  if act[0] == '1' {
+    to, toSize := LZSS.Encode(buffer);
+    
+    /*var j := 0;
+    while j < toSize <= to.Length
+      decreases toSize - j
+    {
+      print(to[j]);
+      j := j+1;
+    }*
+
+    if 0 <= 0 as int <= 0 as int + toSize as int <= to.Length && -0x80000000 <= toSize < 0x80000000 {
+      dstOk := dstFs.Write(0 as nat32, to, 0, toSize as int32);
+    }
+    print "Compress me!\n";
+  } else if act[0] == '0' {
+    to, toSize := LZSS.Decode(buffer);
+    if 0 <= 0 as int <= 0 as int + toSize as int <= to.Length && -0x80000000 <= toSize < 0x80000000 {
+      dstOk := dstFs.Write(0 as nat32, to, 0, toSize as int32);
+    }
+    print "Decompress me!\n";
+  } else {
+    print "[USAGE]: mono compression.exe {0=Compress,1=Decompress} SrcFilename DstFilename!\n";
+  }*/
 }
